coq/proof/SimulationValid.v
@@ -214,7 +214,7 @@ Proof.
     exploit InvState.Rel.inject_value_spec; eauto.
     { rewrite InvState.Unary.sem_valueT_physical. eauto. }
     rewrite InvState.Unary.sem_valueT_physical. s. i. des.
-    eapply _sim_local_step.
+    eapply _sim_local_step; swap 2 3.
     {
       expl progress.
       - ss.
@@ -222,6 +222,7 @@ Proof.
         des_ifs; des; ss.
       - ii. ss.
     }
+    { splits; ss. }
     i.
     expl preservation.
     clear ERROR_SRC.
@@ -366,7 +367,7 @@ Proof.
     clears invst.
     rename STATE0 into STATE1.
     exploit nerror_nfinal_nstuck; eauto. i. des. inv x0.
-    eapply _sim_local_step.
+    eapply _sim_local_step; swap 2 3.
     {
       expl progress.
       - ss.
@@ -374,6 +375,7 @@ Proof.
         des_ifs; des; ss.
       - ii. ss.
     }
+    { split; ss. }
     i.
     expl preservation.
     clear ERROR_SRC.
@@ -445,7 +447,7 @@ Proof.
     clears invst.
     rename STATE0 into STATE1.
     exploit nerror_nfinal_nstuck; eauto. i. des. inv x0.
-    eapply _sim_local_step.
+    eapply _sim_local_step; swap 2 3.
     {
       expl progress.
       - ss.
@@ -453,6 +455,7 @@ Proof.
         des_ifs; des; ss.
       - ii. ss.
     }
+    { split; ss. }
     i.
     expl preservation.
     clear ERROR_SRC.
@@ -1069,17 +1072,17 @@ Lemma valid_init
       (MEM: InvMem.Rel.sem conf_src conf_tgt mem_src mem_tgt inv)
       (CONF: InvState.valid_conf m_src m_tgt conf_src conf_tgt)
       (INIT_SRC: init_fdef conf_src fdef_src args_src ec_src)
-      (WF_TGT: wf_ConfigI conf_tgt)
   :
   exists ec_tgt,
-    <<INIT_TGT: init_fdef conf_tgt fdef_tgt args_tgt ec_tgt>> /\
-    <<SIM:
-      valid_state_sim
-        conf_src conf_tgt
-        stack0_src stack0_tgt
-        inv idx
-        (mkState ec_src stack0_src mem_src)
-        (mkState ec_tgt stack0_tgt mem_tgt)>>.
+    (<<INIT_TGT: init_fdef conf_tgt fdef_tgt args_tgt ec_tgt>>) /\
+    (forall (WF_TGT: wf_ConfigI conf_tgt /\ wf_StateI conf_tgt (mkState ec_tgt stack0_tgt mem_tgt)),
+        <<SIM:
+          valid_state_sim
+            conf_src conf_tgt
+            stack0_src stack0_tgt
+            inv idx
+            (mkState ec_src stack0_src mem_src)
+            (mkState ec_tgt stack0_tgt mem_tgt)>>).
 Proof.
   inv INIT_SRC. unfold valid_fdef in FDEF. simtac.
   exploit locals_init; eauto; [by apply CONF|apply MEM|]. i. des.
@@ -1103,7 +1106,7 @@ Proof.
     s. eauto.
   }
   i. des.
-  esplits.
+  esplits. i; des. splits.
   - econs; eauto. ss.
   - econs; eauto.
     { ss.
@@ -1136,11 +1139,7 @@ Proof.
       cbn in *.
       econs; eauto.
     }
-    {
-      splits; ss.
-      admit.
-    }
-Admitted.
+Qed.
 
 Lemma valid_sim_fdef
       m_src m_tgt
@@ -1154,8 +1153,8 @@ Lemma valid_sim_fdef
   sim_fdef conf_src conf_tgt fdef_src fdef_tgt.
 Proof.
   ii.
-  exploit valid_init; eauto. i. des.
-  esplits; eauto.
+  exploit valid_init; eauto. intro VALID_INIT. des.
+  esplits; eauto. i. specialize (VALID_INIT0 WF_TGT0). des.
   apply valid_sim; eauto.
 Grab Existential Variables.
   { exact 0%nat. }
